theory/x64DecodeProof.thy
@@ -317,7 +317,133 @@ lemma x64_encode_decode_consistency:
     x64_decode pc l = Some (length l_bin, ins)"
   apply (cases ins; simp_all)
 
-  prefer 5
+  prefer 8
+  subgoal for test dst src
+    \<comment> \<open> Pcmovl \<close> 
+    apply (unfold Let_def construct_rex_to_u8_def construct_modsib_to_u8_def)
+    apply (cases test; simp)
+    subgoal by (cases dst; simp; cases src, simp_all add: x64_decode_def bitfield_insert_u8_def
+          Let_def ireg_of_u8_def cond_of_u8_def  Suc3_eq_add_3 add.commute)
+    subgoal
+      by (cases dst; simp; cases src, simp_all add: x64_decode_def bitfield_insert_u8_def
+          Let_def ireg_of_u8_def cond_of_u8_def  Suc3_eq_add_3 add.commute)
+    subgoal by (cases dst; simp; cases src, simp_all add: x64_decode_def bitfield_insert_u8_def
+          Let_def ireg_of_u8_def cond_of_u8_def  Suc3_eq_add_3 add.commute)
+    subgoal
+      by (cases dst; simp; cases src, simp_all add: x64_decode_def bitfield_insert_u8_def
+          Let_def ireg_of_u8_def cond_of_u8_def  Suc3_eq_add_3 add.commute)
+    subgoal by (cases dst; simp; cases src, simp_all add: x64_decode_def bitfield_insert_u8_def
+          Let_def ireg_of_u8_def cond_of_u8_def  Suc3_eq_add_3 add.commute)
+    subgoal
+      by (cases dst; simp; cases src, simp_all add: x64_decode_def bitfield_insert_u8_def
+          Let_def ireg_of_u8_def cond_of_u8_def  Suc3_eq_add_3 add.commute)
+
+    subgoal by (cases dst; simp; cases src, simp_all add: x64_decode_def bitfield_insert_u8_def
+          Let_def ireg_of_u8_def cond_of_u8_def  Suc3_eq_add_3 add.commute)
+    subgoal
+      by (cases dst; simp; cases src, simp_all add: x64_decode_def bitfield_insert_u8_def
+          Let_def ireg_of_u8_def cond_of_u8_def  Suc3_eq_add_3 add.commute)
+
+    subgoal by (cases dst; simp; cases src, simp_all add: x64_decode_def bitfield_insert_u8_def
+          Let_def ireg_of_u8_def cond_of_u8_def  Suc3_eq_add_3 add.commute)
+    subgoal
+      by (cases dst; simp; cases src, simp_all add: x64_decode_def bitfield_insert_u8_def
+          Let_def ireg_of_u8_def cond_of_u8_def  Suc3_eq_add_3 add.commute)
+
+    subgoal by (cases dst; simp; cases src, simp_all add: x64_decode_def bitfield_insert_u8_def
+          Let_def ireg_of_u8_def cond_of_u8_def  Suc3_eq_add_3 add.commute)
+    subgoal
+      by (cases dst; simp; cases src, simp_all add: x64_decode_def bitfield_insert_u8_def
+          Let_def ireg_of_u8_def cond_of_u8_def  Suc3_eq_add_3 add.commute)
+
+    subgoal by (cases dst; simp; cases src, simp_all add: x64_decode_def bitfield_insert_u8_def
+          Let_def ireg_of_u8_def cond_of_u8_def  Suc3_eq_add_3 add.commute)
+    subgoal
+      by (cases dst; simp; cases src, simp_all add: x64_decode_def bitfield_insert_u8_def
+          Let_def ireg_of_u8_def cond_of_u8_def  Suc3_eq_add_3 add.commute)
+
+    subgoal by (cases dst; simp; cases src, simp_all add: x64_decode_def bitfield_insert_u8_def
+          Let_def ireg_of_u8_def cond_of_u8_def  Suc3_eq_add_3 add.commute)
+    subgoal
+      by (cases dst; simp; cases src, simp_all add: x64_decode_def bitfield_insert_u8_def
+          Let_def ireg_of_u8_def cond_of_u8_def  Suc3_eq_add_3 add.commute)
+
+    subgoal by (cases dst; simp; cases src, simp_all add: x64_decode_def bitfield_insert_u8_def
+          Let_def ireg_of_u8_def cond_of_u8_def  Suc3_eq_add_3 add.commute)
+    subgoal
+      by (cases dst; simp; cases src, simp_all add: x64_decode_def bitfield_insert_u8_def
+          Let_def ireg_of_u8_def cond_of_u8_def  Suc3_eq_add_3 add.commute)
+
+    subgoal by (cases dst; simp; cases src, simp_all add: x64_decode_def bitfield_insert_u8_def
+          Let_def ireg_of_u8_def cond_of_u8_def  Suc3_eq_add_3 add.commute)
+    subgoal
+      by (cases dst; simp; cases src, simp_all add: x64_decode_def bitfield_insert_u8_def
+          Let_def ireg_of_u8_def cond_of_u8_def  Suc3_eq_add_3 add.commute)
+
+    subgoal by (cases dst; simp; cases src, simp_all add: x64_decode_def bitfield_insert_u8_def
+          Let_def ireg_of_u8_def cond_of_u8_def  Suc3_eq_add_3 add.commute)
+    subgoal
+      by (cases dst; simp; cases src, simp_all add: x64_decode_def bitfield_insert_u8_def
+          Let_def ireg_of_u8_def cond_of_u8_def  Suc3_eq_add_3 add.commute)
+
+    subgoal by (cases dst; simp; cases src, simp_all add: x64_decode_def bitfield_insert_u8_def
+          Let_def ireg_of_u8_def cond_of_u8_def  Suc3_eq_add_3 add.commute)
+    subgoal
+      by (cases dst; simp; cases src, simp_all add: x64_decode_def bitfield_insert_u8_def
+          Let_def ireg_of_u8_def cond_of_u8_def  Suc3_eq_add_3 add.commute)
+    done
+
+
+
+
+                         
+
+(*proof done
+
+
+  subgoal for dst src
+  \<comment> \<open> Pmovl_rr \<close> 
+    apply (unfold Let_def)
+    apply (cases "construct_rex_to_u8 False (and (u8_of_ireg src) 8 \<noteq> 0) False (and (u8_of_ireg dst) 8 \<noteq> 0) = 64"; simp_all add: construct_rex_to_u8_def construct_modsib_to_u8_def; erule conjE)
+    subgoal by (cases src; cases dst; auto simp add: x64_decode_def bitfield_insert_u8_def Let_def ireg_of_u8_def)
+    subgoal by (cases src; cases dst; auto simp add: x64_decode_def bitfield_insert_u8_def Let_def ireg_of_u8_def)
+    done
+
+  subgoal for dst src
+  \<comment> \<open> Pmovq_rr \<close> 
+    apply (unfold Let_def construct_rex_to_u8_def construct_modsib_to_u8_def; erule conjE; erule conjE)
+    subgoal by (cases src; cases dst; auto simp add: x64_decode_def bitfield_insert_u8_def Let_def ireg_of_u8_def)
+    done
+
+  subgoal for dst imm
+  \<comment> \<open> Pmovl_ri  \<close>
+    apply (unfold Let_def)
+    apply (cases "construct_rex_to_u8 False False False (and (u8_of_ireg dst) 8 \<noteq> 0) = 64";
+        simp_all add:construct_rex_to_u8_def construct_modsib_to_u8_def; erule conjE)
+    subgoal \<comment> \<open> rex = 0x40  \<close>
+      using list_in_list_u8_list_of_u32_simp_sym [of imm "(Suc (Suc pc))" l]
+      using length_u8_list_of_u32_eq_4
+      apply (cases dst; auto simp add: x64_decode_def bitfield_insert_u8_def Let_def
+          ireg_of_u8_def Suc3_eq_add_3 add.commute)
+      done
+
+    subgoal \<comment> \<open> rex <> 0x40  \<close>
+      using list_in_list_u8_list_of_u32_simp_sym [of imm "(pc+3)" l]
+      using length_u8_list_of_u32_eq_4
+      apply (cases dst; auto simp add: x64_decode_def bitfield_insert_u8_def Let_def
+          ireg_of_u8_def Suc3_eq_add_3 add.commute)
+      done
+    done
+
+  subgoal for dst imm
+ \<comment> \<open> Pmovq_ri\<close>
+    apply (unfold Let_def construct_rex_to_u8_def construct_modsib_to_u8_def)
+    using list_in_list_u8_list_of_u64_simp_sym [of imm "(Suc (Suc pc))" l]
+    using length_u8_list_of_u64_eq_8
+    apply (cases dst; simp_all add: bitfield_insert_u8_def x64_decode_def ireg_of_u8_def Suc3_eq_add_3 add.commute)
+    done
+
+      
   subgoal for dst addr chunk
   \<comment> \<open> Pmov_rm \<close>
     apply (cases addr, simp)
@@ -367,129 +493,84 @@ lemma x64_encode_decode_consistency:
           done *)
 
         subgoal \<comment> \<open> ofs > u8 /\ index2 = None  /\ has rex \<close>
-
+          sorry
+(*
           apply (cases chunk; simp; erule conjE; erule conjE; erule conjE)
           apply (unfold construct_rex_to_u8_def construct_modsib_to_u8_def
               bitfield_insert_u8_def Let_def)
-          subgoal
+          subgoal  \<comment> \<open> M32 \<close>
             using list_in_list_u8_list_of_u32_simp_sym [of ofs "(Suc (Suc (Suc pc)))" l]
             using length_u8_list_of_u32_eq_4
-
             apply (cases dst; simp; cases base_reg; simp add: x64_decode_def Let_def ireg_of_u8_def
                     bitfield_insert_u8_def Suc3_eq_add_3 Suc4_eq_add_4 add.commute)
+            done
+          subgoal  \<comment> \<open> M64 \<close>
+            using list_in_list_u8_list_of_u32_simp_sym [of ofs "(Suc (Suc (Suc pc)))" l]
+            using length_u8_list_of_u32_eq_4
+            apply (cases dst; simp; cases base_reg; simp add: x64_decode_def Let_def ireg_of_u8_def
+                    bitfield_insert_u8_def Suc3_eq_add_3 Suc4_eq_add_4 add.commute)
+            done*)
+
+        subgoal for index22\<comment> \<open> index2 = Some \<close>
+          sorry  (*not done*)
+        (*  apply(cases chunk; cases index22;simp_all)
+          subgoal for index_reg scale
+            apply (erule conjE; erule conjE; erule conjE; erule conjE)
+            using list_in_list_u8_list_of_u32_simp_sym [of "ofs" " (Suc (Suc (Suc (Suc pc))))" l]
+            using length_u8_list_of_u32_eq_4
+            using construct_modsib_to_u8_imply_index_reg [of index_reg base_reg "l ! pc" scale "l ! (Suc (Suc (Suc pc)))"]
+            using construct_modsib_to_u8_imply_base_reg [of index_reg base_reg "l ! pc" scale "l ! (Suc (Suc (Suc pc)))"]
+            using construct_modsib_to_u8_imply_scale [of scale index_reg base_reg "l !  Suc (Suc (Suc pc))"]
+            apply (cases dst;simp)
+            subgoal by (cases base_reg; simp; cases index_reg; simp add: construct_rex_to_u8_def construct_modsib_to_u8_def
+                    x64_decode_def bitfield_insert_u8_def Let_def ireg_of_u8_def
+                    add.commute Suc3_eq_add_3 Suc4_eq_add_4) 
+            subgoal by (cases base_reg; simp; cases index_reg; simp add: construct_rex_to_u8_def construct_modsib_to_u8_def
+                    x64_decode_def bitfield_insert_u8_def Let_def ireg_of_u8_def
+                    add.commute Suc3_eq_add_3 Suc4_eq_add_4) *)
+
+            done
           done
+        done
 
-
-        subgoal \<comment> \<open> index2 = Some \<close>
-          apply (cases chunk; simp)
-          apply (unfold construct_rex_to_u8_def construct_modsib_to_u8_def
-              bitfield_insert_u8_def Let_def)
-          apply (cases dst; simp; cases base_reg; simp add: x64_decode_def Let_def ireg_of_u8_def
-                bitfield_insert_u8_def)
-
-          done
-
-
-    apply (unfold Let_def)
-    apply (cases chunk, simp_all)
-      apply (cases base, s- 128 \<le> ofsimp_all)
-      subgoal for base_reg by (cases index2, simp_all)
-      subgoal for base_reg by (cases index2, simp_all)
-      subgoal for base_reg by (cases index2, simp_all)
-      subgoal for base_reg by (cases index2, simp_all)
-      done
-
-    subgoal for base index2 ofs
-      apply (cases base, simp_all)
-      subgoal for base_reg by (cases index2, simp_all)
-      subgoal for base_reg by (cases index2, simp_all)
-      subgoal for base_reg by (cases index2, simp_all)
-      subgoal for base_reg by (cases index2, simp_all)
-      done
-
-    subgoal for base index2 ofs
-      apply (cases base, simp_all)
-      subgoal for base_reg 
-        apply (cases index2, simp_all)
-        subgoal
-          apply (erule conjE;erule conjE)
-          apply (cases dst)
-          subgoal
-            apply simp
-            apply (simp add: construct_rex_to_u8_def bitfield_insert_u8_def Let_def ireg_of_u8_def
-                construct_modsib_to_u8_def)
-            apply (cases base_reg, simp add: x64_decode_def Let_def ireg_of_u8_def  bitfield_insert_u8_def)
-
-
-
-
-
-
-(*proof done
-
-
-  subgoal for dst src
-  \<comment> \<open> Pmovl_rr \<close> 
-    apply (unfold Let_def)
-    apply (cases "construct_rex_to_u8 False (and (u8_of_ireg src) 8 \<noteq> 0) False (and (u8_of_ireg dst) 8 \<noteq> 0) = 64"; simp_all add: construct_rex_to_u8_def construct_modsib_to_u8_def; erule conjE)
-    subgoal by (cases src; cases dst; auto simp add: x64_decode_def bitfield_insert_u8_def Let_def ireg_of_u8_def)
-    subgoal by (cases src; cases dst; auto simp add: x64_decode_def bitfield_insert_u8_def Let_def ireg_of_u8_def)
-    done
-
-  subgoal for dst src
-  \<comment> \<open> Pmovq_rr \<close> 
-    apply (unfold Let_def construct_rex_to_u8_def construct_modsib_to_u8_def; erule conjE; erule conjE)
-    subgoal by (cases src; cases dst; auto simp add: x64_decode_def bitfield_insert_u8_def Let_def ireg_of_u8_def)
-    done
-
-  subgoal for dst imm
-  \<comment> \<open> Pmovl_ri  \<close>
-    apply (unfold Let_def)
-    apply (cases "construct_rex_to_u8 False False False (and (u8_of_ireg dst) 8 \<noteq> 0) = 64";
-        simp_all add:construct_rex_to_u8_def construct_modsib_to_u8_def; erule conjE)
-    subgoal \<comment> \<open> rex = 0x40  \<close>
-      using list_in_list_u8_list_of_u32_simp_sym [of imm "(Suc (Suc pc))" l]
-      using length_u8_list_of_u32_eq_4
-      apply (cases dst; auto simp add: x64_decode_def bitfield_insert_u8_def Let_def
-          ireg_of_u8_def Suc3_eq_add_3 add.commute)
-      done
-
-    subgoal \<comment> \<open> rex <> 0x40  \<close>
-      using list_in_list_u8_list_of_u32_simp_sym [of imm "(pc+3)" l]
-      using length_u8_list_of_u32_eq_4
-      apply (cases dst; auto simp add: x64_decode_def bitfield_insert_u8_def Let_def
-          ireg_of_u8_def Suc3_eq_add_3 add.commute)
-      done
-    done
-
-  subgoal for dst imm
- \<comment> \<open> Pmovq_ri\<close>
-    apply (unfold Let_def construct_rex_to_u8_def construct_modsib_to_u8_def)
-    using list_in_list_u8_list_of_u64_simp_sym [of imm "(Suc (Suc pc))" l]
-    using length_u8_list_of_u64_eq_8
-    apply (cases dst; simp_all add: bitfield_insert_u8_def x64_decode_def ireg_of_u8_def Suc3_eq_add_3 add.commute)
-    done
-
-      
-  subgoal for dst src chunk
-  \<comment> \<open> Pmov_rm 
-    apply (cases dst, simp)
-    subgoal for rd rs ro
-      apply (cases rd, simp_all)
-      subgoal for rd1
-        apply (cases rs, simp_all)
-        apply (cases "rd1 = ireg.R11 \<and> ro = 0", simp_all add: Let_def)
-        apply (unfold Let_def construct_rex_to_u8_def construct_modsib_to_u8_def)
-        apply (cases chunk; cases src; auto simp add: x64_decode_def bitfield_insert_u8_def Let_def ireg_of_u8_def)\<close> 
-    sorry
 
   subgoal for dst src chunk
     \<comment> \<open> Pmov_mr \<close> 
     sorry
 
-  subgoal for dst imm chunk
+  subgoal for addr imm chunk
     \<comment> \<open> Pmov_mi \<close> 
-    sorry
+    apply(cases chunk, simp_all)
+    apply (cases addr, simp)
+    subgoal for base index2 ofs
+      apply (cases base, simp_all)
+      subgoal for base_reg
+        apply (cases index2; simp add: Let_def; erule conjE; erule conjE; erule conjE; erule conjE)
+        subgoal
+          apply (auto simp add: construct_rex_to_u8_def construct_modsib_to_u8_def)
+          subgoal
+            using list_in_list_u8_list_of_u32_simp_sym [of imm "(Suc (Suc (Suc (Suc pc))))" l]
+            using length_u8_list_of_u32_eq_4 
+            using scast_u32_scast_u8_eq
+              by (cases base_reg;auto simp add: x64_decode_def Let_def ireg_of_u8_def
+                bitfield_insert_u8_def Suc3_eq_add_3 Suc4_eq_add_4 add.commute)
+            subgoal
+            using list_in_list_u8_list_of_u32_simp_sym [of imm "(Suc (Suc (Suc (Suc pc))))" l]
+            using length_u8_list_of_u32_eq_4 
+            using scast_u32_scast_u8_eq
+            by (cases base_reg;auto simp add: x64_decode_def Let_def ireg_of_u8_def
+                bitfield_insert_u8_def Suc3_eq_add_3 Suc4_eq_add_4 add.commute)
+          done
+        subgoal
+          apply (simp add: list_in_list_concat length_u8_list_of_u32_eq_4)
+          using list_in_list_u8_list_of_u32_simp_sym [of "ofs" "(Suc (Suc (Suc pc)))" l]
+          using list_in_list_u8_list_of_u32_simp_sym [of imm "(7 + pc)" l]
+          apply (cases base_reg; simp add: x64_decode_def  construct_rex_to_u8_def bitfield_insert_u8_def 
+              Let_def construct_modsib_to_u8_def ireg_of_u8_def Suc3_eq_add_3 Suc4_eq_add_4 add.commute)
+          done
+        done
+      done
+    done
 
   subgoal for test dst src
     \<comment> \<open> Pcmovl \<close> 
